SP1Chips/ShiftRight/Constraints.lean
@@ -607,7 +607,7 @@ lemma register_bounds : List.Forall SP1Constraint.toProp (constraints Main) → 
             b_srl, b_sra, b_srlw, b_sraw, one_of_ops, h4 ⟩ := cstrs
   clear h0 h1 h2 h3 h4
   rw [ALUTypeReader.allHold_constraints_iff_is_real] at alu
-  . obtain ⟨ h0, h1, h2, h3, h4, h5, b_imm, h7, h8, h9, h10, h11, h12, h13, h14, h15, h16, h17, h18, h19 ⟩ := alu
+  . obtain ⟨ h0, h1, h2, h3, h4, h5, _, b_imm, h7, h8, h9, h10, h11, h12, h13, h14, h15, h16, h17, h18 ⟩ := alu
     rcases real with srl | sra | srlw | sraw <;> simp_all [Opcode.ofNat, Nat.ble, Nat.beq] <;>
     rcases b_imm <;> simp_all
   . clear alu; rcases real with srl | sra | srlw | sraw <;> simp_all
@@ -641,7 +641,7 @@ lemma op_a_is_0 : List.Forall SP1Constraint.toProp (constraints Main) → is_rea
             b_srl, b_sra, b_srlw, b_sraw, one_of_ops, h4 ⟩ := cstrs
   clear h0 h1 h2 h3 h4
   rw [ALUTypeReader.allHold_constraints_iff_is_real] at alu
-  . obtain ⟨ h0, h1, h2, h3, h4, h5, b_imm, h7, h8, h9, h10, h11, h12, h13, h14, h15, h16, h17, h18, h19 ⟩ := alu
+  . obtain ⟨ h0, h1, h2, h3, _, h4, h5, b_imm, h7, h8, h9, h10, h11, h12, h13, h14, h15, h16, h17, h18 ⟩ := alu
     clear *- h4 h5 h18; simp_all; aesop
   . clear alu; rcases real with srl | sra | srlw | sraw <;> simp_all
 
@@ -656,7 +656,7 @@ lemma ops_U64_b_c : List.Forall SP1Constraint.toProp (constraints Main) → is_r
           b_srl, b_sra, b_srlw, b_sraw, one_of_ops, h4 ⟩ := cstrs
   clear h0 h1 h2 h3 h4
   rw [ALUTypeReader.allHold_constraints_iff_is_real] at alu
-  . obtain ⟨ h0, h1, h2, h3, h4, h5, b_imm, h7, h8, h9, h10, h11, h12, h13, h14, h15, h16, h17, h18, h19 ⟩ := alu
+  . obtain ⟨ h0, h1, h2, h3, _, h4, h5, b_imm, h7, h8, h9, h10, h11, h12, h13, h14, h15, h16, h17, h18 ⟩ := alu
     rcases real with srl | sra | srlw | sraw <;> simp_all [Opcode.ofNat, Nat.ble, Nat.beq] <;>
     rcases b_imm <;> simp_all <;> apply Word.isU64_of_cases <;> simp <;> omega
   . clear alu; rcases real with srl | sra | srlw | sraw <;> simp_all
